Created run.sh executable

website/Walkthrough/Blog/Introduction.lean
@@ -11,80 +11,8 @@ date := {year := 2024, month := 1, day := 15}
 This is a tutorial on metaprogramming, or equivalently, writing tactics to help prove math theorems, in Lean 4.
 That is, instead of focusing on writing a _formalized proof_ (programming), we focus on writing a _program that writes a formalized proof_ (metaprogramming).
 
-```leanInit demo
--- This block initializes a Lean context
-```
+# Code
+- Here is the [full code](http://google.com) containing everything in the tutorial.
+- Here is a [short "cheet sheet"](http://google.com) containing helper functions you might find useful when metaprogramming in the future.
 
-
-```lean demo
-example := if true then 1 else 2
-example := if True then 1 else 2
-example : Int := if True then 1 else 2
-```
-
-```lean demo
-/-- A recursive function -/
-def slowId : Nat → Nat
-  | 0 => 0
-  | n + 1 => slowId n + 1
-
-#eval slowId 5
-
-/-- An array literal -/
-example := #[1, 2, 3]
-
-example := 33
-```
-
-I can also prove things about conditionals!
-```lean demo
-theorem lt_4 (b : Bool) : (if b then 1 else 2) < 4 := by
-  split
-  . skip; decide
-  . decide
-```
-
-It's also nice to write normal proofs sometimes.
-
-```lean demo
-def rev : List α → List α
-  | [] => []
-  | x :: xs => rev xs ++ [x]
-
-def revAcc (acc : List α) : List α → List α
-  | [] => acc
-  | x :: xs => revAcc (x :: acc) xs
-
-theorem rev_append_eq_revAcc (acc xs : List α) :
-    rev xs ++ acc = revAcc acc xs := by
-  induction xs generalizing acc with
-  | nil => simp [rev, revAcc]
-  | cons x xs ih =>
-    unfold rev
-    unfold revAcc
-    rw [List.append_assoc]
-    apply ih
-```
-
-Here are some uses of various constructors:
-```lean demo
-def squish (n : Option Nat) : Nat :=
-  match n with
-  | none => 0
-  | some k => .succ k
-
-def squish' (n : Option Nat) : Nat :=
-  match n with
-  | .none => 0
-  | .some k => k.succ
-
-open Nat in
-def squish'' (n : Option Nat) : Nat :=
-  match n with
-  | none => 0
-  | some k => succ k
-
-```
-
-
-Thank you for looking at my test/demo post.
+# Looking Ahead
