run.sh
@@ -1,0 +1,3 @@
+lake build
+lake exe walkthrough --output _out/walkthroughsite
+python3 -m http.server 8800 --directory _out/walkthroughsite
